src/crypto_foundations/computational_monads/random_oracle.lean
@@ -1,6 +1,16 @@
 import crypto_foundations.computational_monads.oracle_comp
 
-/-- Oracle access to a random function -/
+def random_simulation {T U C : Type} 
+  [decidable_eq T] [fintype U] [inhabited U]
+  (oc : oracle_comp.singleton_oracle_comp T U C) : 
+  comp (C × list (T × U)) :=
+oc.simulate [] (λ _ log t, 
+option.rec_on (log.find (λ tu, t = tu.1)) 
+  -- If this isn't in the query log, return a random output and add that to the log
+  (comp.bind (comp.rnd U) (λ u, comp.ret ⟨u, ⟨t, u⟩ :: log⟩))
+  (λ tu, comp.ret ⟨tu.2, log⟩))
+
+/-- Oracle access to a uniformly random function `T → U` -/
 def random_oracle_comp (T U : Type) [decidable_eq T]
   [fintype U] [inhabited U] :=
 oracle_comp.singleton_oracle_comp T U
@@ -8,10 +18,21 @@ oracle_comp.singleton_oracle_comp T U
 variables {T U : Type}
   [decidable_eq T] [fintype U] [inhabited U]
 
-def random_oracle_comp.eval_distribution {C : Type}
-  (roc : random_oracle_comp T U C) : comp (C × list (T × U)) :=
-roc.eval_distribution [] (λ _ log t, 
+@[derive comp.is_well_formed]
+def random_oracle_comp.simulate {C : Type}
+  (roc : random_oracle_comp T U C) [roc.is_well_formed]
+  (log_init : list (T × U)) : comp (C × list (T × U)) :=
+roc.simulate log_init (λ _ log t, 
 option.rec_on (log.find (λ tu, t = tu.1)) 
   -- If this isn't in the query log, return a random output and add that to the log
   (comp.bind (comp.rnd U) (λ u, comp.ret ⟨u, ⟨t, u⟩ :: log⟩))
   (λ tu, comp.ret ⟨tu.2, log⟩))
+
+-- @[simp]
+-- instance random_oracle_comp.simulate.is_well_formed {C : Type}
+--   (roc : random_oracle_comp T U C) [roc.is_well_formed]
+--   (log_init : list (T × U)) :
+--   (roc.simulate log_init).is_well_formed :=
+-- begin
+--   simp [random_oracle_comp.simulate],
+-- end
