src/crypto_foundations/primitives/signature/signature.lean
@@ -1,0 +1,101 @@
+import crypto_foundations.computational_monads.dist_sem
+import crypto_foundations.computational_monads.vector_call
+import crypto_foundations.computational_monads.random_oracle
+import computational_complexity.complexity_class
+import computational_complexity.negligable
+import data.list.basic
+
+structure signature (M PK SK S ROI ROO : Type)
+  [decidable_eq M] [decidable_eq PK]
+  [decidable_eq ROI] [fintype ROO]
+  [inhabited ROO] :=
+(gen : unit → comp (PK × SK))
+(gen_is_well_formed : ∀ x, (gen x).is_well_formed)
+(sign : SK × M → random_oracle_comp ROI ROO S)
+(sign_is_well_formed : ∀ x, (sign x).is_well_formed)
+(verify : PK × S → random_oracle_comp ROI ROO bool)
+(verify_is_well_formed : ∀ x, (verify x).is_well_formed)
+
+namespace signature
+
+variables {M PK SK S ROI ROO : Type}
+  [decidable_eq M] [decidable_eq PK]
+  [decidable_eq ROI] [fintype ROO]
+  [inhabited ROO]
+variable (sig : signature M PK SK S ROI ROO)
+
+section is_well_formed_instances
+
+@[simp]
+instance gen.is_well_formed (u : unit) :
+  (sig.gen u).is_well_formed :=
+sig.gen_is_well_formed _
+
+@[simp]
+instance sign.is_well_formed (inp : SK × M) :
+  (sig.sign inp).is_well_formed :=
+sig.sign_is_well_formed _
+
+@[simp]
+instance verify.is_well_formed (inp : PK × S) :
+  (sig.verify inp).is_well_formed :=
+sig.verify_is_well_formed _
+
+end is_well_formed_instances
+
+section complete
+
+def completeness_experiment (m : M) : comp bool :=
+do (pk, sk) ← sig.gen (),
+  (σ, log) ← (sig.sign (sk, m)).simulate [],
+  (b, _) ← (sig.verify (pk, σ)).simulate log,
+  return b
+
+@[simp]
+-- TODO: I think it should be possible to write a derive handler for this
+instance comleteness_experiment.is_well_formed (m : M) : 
+  (completeness_experiment sig m).is_well_formed :=
+by simp [completeness_experiment]
+
+@[simp]
+lemma mem_completeness_experiment_iff (m : M) (b : bool) :
+  b ∈ (completeness_experiment sig m).support ↔
+    ∃ (pk : PK) (sk : SK) (hks : (pk, sk) ∈ (sig.gen ()).support)
+      (σ : S) log (hσ : (σ, log) ∈ ((sig.sign (sk, m)).simulate []).support)
+      (b' : bool) log' (hb' : (b', log') ∈ ((sig.verify (pk, σ)).simulate log).support),
+      b = b' :=
+by simp [completeness_experiment]
+
+def complete :=
+∀ (m : M), (completeness_experiment sig m).Pr = 1
+
+end complete
+
+end signature
+
+variables [function_cost_model ℚ] [comp_cost_model ℚ]
+
+structure signature_scheme (M : Type) (PK SK S ROI ROO : ℕ → Type)
+  [decidable_eq M] [∀ sp, decidable_eq $ PK sp]
+  [∀ sp, decidable_eq $ ROI sp] [∀ sp, fintype $ ROO sp]
+  [∀ sp, inhabited $ ROO sp] :=
+(sig (sp : ℕ) : signature M (PK sp) (SK sp) (S sp) (ROI sp) (ROO sp))
+(gen_polnomial_complexity : complexity_class.polynomial_complexity (λ sp, (sig sp).gen))
+(sign_polynomial_complexity : sorry) --complexity_class.polynomial_complexity (λ sp, (sig sp).sign))
+(verify_polynomial_complexity : sorry)
+
+namespace signature_scheme
+
+variables (M : Type) (PK SK S ROI ROO : ℕ → Type)
+  [decidable_eq M] [∀ sp, decidable_eq $ PK sp]
+  [∀ sp, decidable_eq $ ROI sp] [∀ sp, fintype $ ROO sp]
+  [∀ sp, inhabited $ ROO sp]
+  (sigs : signature_scheme M PK SK S ROI ROO)
+
+section unforgeable
+
+def unforgeable : Prop := sorry
+
+end unforgeable
+
+end signature_scheme
